

5. Prove the estimate (12.23). $\|\tau_h\|_h^2 \leq 3(\|f\|_h^2 + \|f\|_{L^1(\omega)}^2)$
 [Hint: for each internal node x_j , $j = 1, \dots, n-1$, integrate by parts (12.21) to get

$$\tau_h(x_j) = -u''(x_j) - \frac{1}{h^2} \left[\int_{x_j-h}^{x_j} u''(t)(x_j-h-t)^2 dt - \int_{x_j}^{x_j+h} u''(t)(x_j+h-t)^2 dt \right].$$

Then, pass to the squares and sum $\tau_h(x_j)^2$ for $j = 1, \dots, n-1$. On noting that $(a+b+c)^2 \leq 3(a^2+b^2+c^2)$, for any real numbers a, b, c , and applying the Cauchy-Schwarz inequality yields the desired result.]

$$(\|v\|_h := h \sum_{j=1}^{n-1} v(x_j)^2, \quad x_j = jh, \quad h = \frac{1}{n})$$

From (12.21), we have

$$\tau_h(x_j) = \frac{1}{h^2} (R_+(x_j+h) + R_-(x_j-h))$$

where

$$R_+(x_j+h) = \int_{x_j}^{x_j+h} \frac{(u''(t) - u''(x_j))}{2} (x_j+h-t)^2 dt$$

$$R_-(x_j-h) = - \int_{x_j-h}^{x_j} \frac{(u''(t) - u''(x_j))}{2} (x_j-h-t)^2 dt$$

Integrating by parts, we have

$$\tau_h(x_j) = -u''(x_j) - \frac{1}{h^2} \left[\int_{x_j-h}^{x_j} u''(t)(x_j-h-t) dt - \int_{x_j}^{x_j+h} u''(t)(x_j-h-t) dt \right]$$

With $f = -u''$ and define

$$B_j = \frac{1}{h^2} \int_{x_j-h}^{x_j} f(t)(x_j-h-t) dt$$

$$C_j = \frac{1}{h^2} \int_{x_j}^{x_j+h} f(t)(x_j+h-t) dt$$

Then

$$\tau_h(x_j) = f(x_j) + B_j + C_j$$

Using $(a+b+c)^2 \leq 3(a^2+b^2+c^2)$, we have

$$(\tau_h(x_j))^2 \leq 3(f(x_j)^2 + B_j^2 + C_j^2)$$

Multiplying by h and summing over j ,

$$\|\tau_h\|_h^2 = h \sum_{j=1}^{n-1} (\tau_h(x_j))^2 \leq 3\|f\|_h^2 + 3h \sum_{j=1}^{n-1} (B_j^2 + C_j^2)$$

Then it remains to estimate $\sum (B_j^2 + C_j^2)$

By the Cauchy-Schwarz inequality for integral,

$$B_j^2 \leq \frac{1}{h^2} \left(\int_{x_j-h}^{x_j} f(t)^2 dt \right) \left(\int_{x_j-h}^{x_j} (x_j-h-t)^2 dt \right)$$

Since

$$\int_{x_j-h}^{x_j} (x_j-h-t)^2 dt = \int_0^h s^2 ds = \frac{h^3}{3}$$

Then, we obtain

$$B_j^2 \leq \frac{1}{3h} \int_{x_j-h}^{x_j} f(t)^2 dt$$

Similarly,

$$C_j^2 \leq \frac{1}{3h} \int_{x_j}^{x_j+h} f(t)^2 dt$$

Hence,

$$h \sum_{j=1}^{n-1} (B_j^2 + C_j^2) \leq \frac{1}{3} \sum_{j=1}^{n-1} \left(\int_{x_j-h}^{x_j} f^2 + \int_{x_j}^{x_j+h} f^2 \right) \leq \frac{1}{3} \|f\|_{L^1(\omega)}^2 \leq \|f\|_{L^1(\omega)}^2$$

Therefore,

$$\|\tau_h\|_h^2 \leq 3(\|f\|_h^2 + \|f\|_{L^1(\omega)}^2)$$

7. Let $g = 1$ and prove that $T_h g(x_j) = \frac{1}{2}x_j(1-x_j)$. $w_h = T_h g$, $w_h = \sum_{k=1}^{n-1} g(x_k) G^k$
 [Solution: use the definition (12.25) with $g(x_k) = 1$, $k = 1, \dots, n-1$ and recall that $G^k(x_j) = hG(x_j, x_k)$ from the exercise above. Then

$$T_h g(x_j) = h \left[\sum_{k=1}^j x_k(1-x_j) + \sum_{k=j+1}^{n-1} x_j(1-x_k) \right]$$

from which, after straightforward computations, one gets the desired result.]

Since $g(x_k) = 1$ for all k , from (12.25) and problem 6 we have

$$T_h g(x_j) = \sum_{k=1}^{n-1} G^k(x_j) = \sum_{k=1}^{n-1} hG(x_j, x_k) = h \sum_{k=1}^{n-1} G(x_j, x_k) \quad (1)$$

From the form of Green's function, we know that

If $k \leq j$, then $x_k \leq x_j$ and $G(x_j, x_k) = x_k(1-x_j)$

If $k > j$, then $x_k > x_j$ and $G(x_j, x_k) = x_j(1-x_k)$

Thus, (1) becomes

$$T_h g(x_j) = h \left[\sum_{k=1}^j x_k(1-x_j) + \sum_{k=j+1}^{n-1} x_j(1-x_k) \right]$$

Let $x_k = kh$, $h = \frac{1}{n}$, then

$$\sum_{k=1}^j x_k = \sum_{k=1}^j kh = h \frac{j(j+1)}{2}$$

and

$$\sum_{k=1}^j (1-x_k) = \sum_{k=1}^j 1 - h \sum_{k=1}^j k = (j+1) - h \frac{j(j+1)}{2}$$

Furthermore, using $x_j = jh$, $h = \frac{1}{n}$

$$\begin{aligned} T_h g(x_j) &= \frac{1}{n} \left[(1 - \frac{j}{n}) \cdot \frac{1}{n} \cdot \frac{j(j+1)}{2} + \frac{j}{n} \cdot \left((n-1-j) - \frac{1}{n} \left(\frac{(n-1)n}{2} - \frac{j(j+1)}{2} \right) \right) \right] \\ &= \frac{1}{n^2} \left(1 - \frac{j}{n} \right) \cdot \frac{j^2+j}{2} + \frac{j}{n^2} \left((n-1-j) - \frac{1}{n} \left(\frac{n^2-n}{2} - \frac{j^2+j}{2} \right) \right) \\ &= \frac{j^2+j}{2n^2} - \frac{j^3+j^2}{2n^3} + \frac{2nj-2j-zj^2}{2n^2} - \frac{nj-j}{2n^2} + \frac{j^3+j^2}{2n^3} \\ &= \frac{j^2+j-2j-zj^2+j^2}{2n^2} + \frac{2j-j}{2n} = \frac{j}{2n} - \frac{j^2}{2n^2} \end{aligned}$$

and

$$\frac{1}{2}x_j(1-x_j) = \frac{1}{2} \cdot \frac{j}{n} \left(1 - \frac{j}{n} \right) = \frac{j}{2n} - \frac{j^2}{2n^2}$$

Therefore,

$$T_h g(x_j) = \frac{1}{2}x_j(1-x_j), \quad j=1, \dots, n-1$$

8. Prove Young's inequality (12.40). $ab \leq \varepsilon a^2 + \frac{1}{4\varepsilon} b^2, \forall a, b \in \mathbb{R}, \forall \varepsilon > 0$

Let $a, b \in \mathbb{R}$ and $\varepsilon > 0$ be arbitrary.
Consider the square of any real number

$$\sqrt{\varepsilon}a - \frac{1}{\sqrt{4\varepsilon}}b$$

Then we have

$$\left(\sqrt{\varepsilon}a - \frac{1}{\sqrt{4\varepsilon}}b\right)^2 \geq 0$$

$$\Rightarrow \varepsilon a^2 - 2 \cdot \sqrt{\varepsilon}a \cdot \frac{1}{\sqrt{4\varepsilon}}b + \frac{1}{4\varepsilon}b^2 \geq 0$$

$$\Rightarrow \varepsilon a^2 + \frac{1}{4\varepsilon}b^2 \geq ab$$

Therefore, $ab \leq \varepsilon a^2 + \frac{1}{4\varepsilon}b^2$

9. Show that $\|v_h\|_h \leq \|v_h\|_{h,\infty} \forall v_h \in V_h$.

Let $v_h \in V_h$. Recall the discrete norms

$$\|v_h\|_h^2 = h \sum_{j=1}^{n-1} v_h(x_j)^2, \quad \|v_h\|_{h,\infty} = \max_{1 \leq j \leq n-1} |v_h(x_j)|$$

For every j we have

$$|v_h(x_j)| \leq \|v_h\|_{h,\infty} \Rightarrow v_h(x_j)^2 \leq \|v_h\|_{h,\infty}^2$$

Therefore,

$$\|v_h\|_h^2 = h \sum_{j=1}^{n-1} v_h(x_j)^2 \leq h \sum_{j=1}^{n-1} \|v_h\|_{h,\infty}^2 = h(n-1) \|v_h\|_{h,\infty}^2$$

Since the grid is uniform on $[0, 1]$, $h = \frac{1}{n}$ and hence

$$h(n-1) = \frac{n-1}{n} < 1$$

Therefore, $\|v_h\|_h \leq \|v_h\|_{h,\infty}, \forall v_h \in V_h$

11. Discretize the fourth-order differential operator $Lu(x) = -u^{(iv)}(x)$ using centered finite differences.

[Solution: apply twice the second order centered finite difference operator L_h defined in (12.9).]

$Lu(x) = -u^{(iv)}(x)$. Let $u_h = \{u_j\}$ be the grid values $u_j \approx u(x_j)$, $x_j = jh$

Let $v_h = L_h u_h$, then

$$v_j = (L_h u_h)(x_j) = -\frac{u_{j+1} - 2u_j + u_{j-1}}{h^2}$$

Now apply L_h to v_h ,

$$(L_h v_h)(x_j) = -\frac{v_{j+1} - 2v_j + v_{j-1}}{h^2}$$

Substitute the expression of v_{j+1} , v_j , v_{j-1}

$$V_{j+1} = - \frac{U_{j+2} - 2U_{j+1} + U_j}{h^2}$$

$$V_j = - \frac{U_{j+1} - 2U_j + U_{j-1}}{h^2}$$

$$V_{j-1} = - \frac{U_j - 2U_{j-1} + U_{j-2}}{h^2}$$

Hence,

$$(L_h V_h)(x_j) = - \frac{1}{h^2} (V_{j+1} - 2V_j + V_{j-1})$$

$$= - \frac{1}{h^2} \left[- \frac{U_{j+2} - 2U_{j+1} + U_j}{h^2} + 2 \frac{U_{j+1} - 2U_j + U_{j-1}}{h^2} - \frac{U_j - 2U_{j-1} + U_{j-2}}{h^2} \right]$$

$$= \frac{1}{h^4} (U_{j+2} - 4U_{j+1} + 6U_j - 4U_{j-1} + U_{j-2})$$